From20To30/Call.v
@@ -1,0 +1,881 @@
+From Coq Require Import String ZArith NArith Eqdep_dec List Lia.
+
+From Coq Require PropExtensionality.
+
+From Vyper Require Import Config Calldag L10.Base.
+From Vyper Require L20.AST L20.Expr L30.AST L20.Interpret L30.Interpret.
+
+From Vyper.From20To30 Require Import Translate Callset FunCtx Expr Stmt.
+
+Lemma nodup_app {A: Type} (EqDec: forall x y: A, {x = y} + {x <> y})
+                {a b: list A}
+                (NA: NoDup a)
+                (NB: NoDup b)
+                (Disjoint: forall x,
+                             (ListSet.set_mem EqDec x a && ListSet.set_mem EqDec x b = false)%bool):
+  NoDup (a ++ b).
+Proof.
+induction a as [|ha]. { apply NB. }
+cbn. constructor.
+{ (* ~ In ha (a ++ b) *)
+  rewrite in_app_iff.
+  intro H. case H; clear H; intro H.
+  { now inversion NA. }
+  assert (Q := Disjoint ha).
+  cbn in Q. destruct EqDec. 2:tauto.
+  rewrite Bool.andb_true_l in Q.
+  now rewrite ListSet2.set_mem_false in Q.
+}
+apply IHa. { now inversion NA. }
+intro x.
+assert (U := Disjoint x).
+cbn in U.
+destruct EqDec. 2:assumption.
+now destruct (ListSet.set_mem EqDec x a).
+Qed.
+
+Lemma nodup_app_elim_r {A: Type} (EqDec: forall x y: A, {x = y} + {x <> y})
+                       {a b: list A}
+                       (H: NoDup (a ++ b)):
+  NoDup b.
+Proof.
+induction a as [|ha]. { apply H. }
+cbn in H. apply IHa. inversion H. assumption.
+Qed.
+
+Lemma nodup_disjoint {A: Type} (EqDec: forall x y: A, {x = y} + {x <> y})
+                     {a b: list A}
+                     (H: NoDup (a ++ b))
+                     (x: A):
+  (ListSet.set_mem EqDec x a && ListSet.set_mem EqDec x b = false)%bool.
+Proof.
+induction a as [|ha]. { easy. }
+cbn.
+destruct (EqDec x ha). 2:{ inversion H. tauto. }
+subst x.
+rewrite Bool.andb_true_l.
+rewrite ListSet2.set_mem_false.
+cbn in H.
+assert (W: ~ In ha (a ++ b)) by now inversion H.
+rewrite in_app_iff in W. tauto.
+Qed.
+
+Lemma alist_set_mem {A B: Type} (EqDec: forall x y: A, {x = y} + {x <> y})
+                    (x: A) (alist: list (A * B)):
+  ListSet.set_mem EqDec x (map fst alist)
+   =
+  match Map.alist_lookup EqDec alist x with
+  | Some _ => true
+  | None => false
+  end.
+Proof.
+induction alist. { easy. }
+cbn. rewrite IHalist.
+destruct a as (k, v). cbn.
+now destruct (EqDec x k).
+Qed.
+
+Lemma varmap_if_nodup {C: VyperConfig}
+                      (names: list string)
+                      (ND: NoDup names)
+                      (err: string):
+  make_varmap names <> inl err.
+Proof.
+unfold make_varmap.
+pose (empty  := @Map.empty  string string_dec N (@string_map C N) (@string_map_impl C N)).
+pose (items  := @Map.items  string string_dec N (@string_map C N) (@string_map_impl C N)).
+pose (insert := @Map.insert string string_dec N (@string_map C N) (@string_map_impl C N)).
+fold empty.
+assert (ND': NoDup (map fst (items empty) ++ names)).
+{ unfold empty. unfold items. rewrite Map.empty_items. cbn. exact ND. }
+enough (H: forall m n,
+             NoDup (map fst (items m) ++ names)
+              ->
+             make_varmap_rec m n names <> inl err).
+{ apply H. apply ND'. }
+clear ND ND'.
+induction names; intros m n H. { easy. }
+cbn.
+rewrite Map.items_ok.
+destruct (NoDup_remove _ _ _ H) as (H', NotIn).
+rewrite in_app_iff in NotIn.
+rewrite Map.alist_lookup_not_in by tauto.
+apply IHnames.
+(* goal: NoDup (map fst (items (Map.insert m a n)) ++ names) *)
+apply (nodup_app string_dec).
+{ apply Map.items_nodup. }
+{ apply (nodup_app_elim_r string_dec H'). }
+(* disjoint *)
+intro x.
+assert (D := nodup_disjoint string_dec H x).
+cbn in D.
+assert (F: ListSet.set_mem string_dec x (map fst (items (insert m a n)))
+            =
+           if string_dec x a then true else ListSet.set_mem string_dec x (map fst (items m))).
+{
+  repeat rewrite alist_set_mem. unfold items. repeat rewrite<- Map.items_ok.
+  unfold insert. rewrite Map.insert_ok.
+  destruct (string_dec a x), (string_dec x a); now subst.
+}
+fold insert. rewrite F. clear F.
+destruct (ListSet.set_mem string_dec x (map fst (items m))), (string_dec x a); try easy.
+rewrite Bool.andb_true_l.
+rewrite ListSet2.set_mem_false.
+subst x. tauto.
+Qed.
+
+Lemma varmap_rec_not_in {C: VyperConfig}
+                        (a: string)
+                        (names: list string)
+                        (m: string_map N)
+                        (init: N)
+                        (L: let _ := string_map_impl in Map.lookup m a <> None)
+                        (Ok: forall err, make_varmap_rec m init names <> inl err):
+  ~ In a names.
+Proof.
+pose (insert := @Map.insert string string_dec N (@string_map C N) (@string_map_impl C N)).
+revert m init L Ok. induction names as [|head]; intros. { easy. }
+cbn in *.
+remember (Map.lookup m head) as m_head. destruct m_head.
+{ exfalso. exact (Ok _ eq_refl). }
+assert (NE: head <> a).
+{ intro. subst. rewrite<- Heqm_head in L. tauto. }
+enough (~ In a names) by tauto.
+apply (IHnames (insert m head init) (N.succ init)).
+2: apply Ok.
+unfold insert.
+rewrite Map.insert_ok.
+now destruct (string_dec head a).
+Qed.
+
+Lemma varmap_rec_cons {C: VyperConfig}
+                      (head: string)
+                      (tail: list string)
+                      (m: string_map N)
+                      (init: N)
+                      (Ok: forall err, make_varmap_rec m init (head :: tail) <> inl err):
+  ~ In head tail.
+Proof.
+cbn in Ok.
+destruct (Map.lookup m head). { exfalso. exact (Ok _ eq_refl). }
+refine (varmap_rec_not_in head tail _ _ _ Ok).
+cbn. rewrite Map.insert_ok.
+now destruct (string_dec head head).
+Qed.
+
+(** If [make_varmap names] finished successfully, then there's no duplicates in [names]. *)
+Lemma varmap_nodup {C: VyperConfig}
+                   (names: list string)
+                   (Ok: forall err, make_varmap names <> inl err):
+  NoDup names.
+Proof.
+unfold make_varmap in Ok.
+pose (empty  := @Map.empty  string string_dec N (@string_map C N) (@string_map_impl C N)).
+pose (items  := @Map.items  string string_dec N (@string_map C N) (@string_map_impl C N)).
+pose (insert := @Map.insert string string_dec N (@string_map C N) (@string_map_impl C N)).
+pose (lookup := @Map.lookup string string_dec N (@string_map C N) (@string_map_impl C N)).
+fold empty in Ok.
+enough (H: forall (m: string_map N)
+               (init: N)
+               (Disjoint: forall x,
+                            match lookup m x with
+                            | Some _ => ~ In x names
+                            | None => True
+                            end)
+               (Success: forall err, make_varmap_rec m init names <> inl err),
+            NoDup names).
+{
+  apply (H empty 0%N); try assumption.
+  unfold lookup. unfold empty. intro x. now rewrite Map.empty_lookup.
+}
+clear Ok.
+induction names. { constructor. }
+intros.
+assert (V := varmap_rec_cons a names m init Success).
+cbn in Success.
+remember (Map.lookup m a) as ma.
+destruct ma. { exfalso. exact (Success "duplicate argument name"%string eq_refl). }
+constructor. { exact V. }
+refine (IHnames (insert m a init) (N.succ init) _ Success).
+intro x.
+unfold lookup in *. unfold insert. rewrite Map.insert_ok.
+cbn in Disjoint. assert (Dx := Disjoint x).
+destruct (string_dec a x). { now subst. }
+destruct (Map.lookup m x); tauto.
+Qed.
+
+
+(** Given that [names] and [values] have the same length and there is no duplication in [names],
+    [bind_args] computes successfully and returns a map that is only defined on strings from [names].
+ *)
+Lemma bind_args_domain_if_nodup {C: VyperConfig}
+                                (names: list string)
+                                (values: list uint256)
+                                (SameLen: length names = length values)
+                                (ND: NoDup names):
+  let _ := string_map_impl in
+  match L10.Interpret.bind_args names values with
+  | inl err => False
+  | inr m => forall x,
+               match Map.lookup m x with
+               | None => ~ In x names
+               | Some _ => In x names
+               end
+  end.
+Proof.
+revert values SameLen. induction names, values; try easy.
+{ cbn. intro H. clear H. intro x. now rewrite Map.empty_lookup. }
+cbn. intro SameLen'.
+assert (L: length names = length values) by now inversion SameLen'. clear SameLen'.
+assert (ND_names: NoDup names) by now inversion ND.
+assert (IH := IHnames ND_names values L).
+destruct (Interpret.bind_args names values). { exact IH. }
+assert (A := IH a). destruct (Map.lookup s a). { now inversion ND. }
+intro x.
+assert (X := IH x). rewrite Map.insert_ok.
+destruct (string_dec a x). { now left. }
+destruct Map.lookup; tauto.
+Qed.
+
+(** This is a variant of [bind_args_domain_if_nodup] but it directly assumes
+    successful completion of [bind_args] instead of preconditions. *)
+Lemma bind_args_domain {C: VyperConfig}
+                   (names: list string)
+                   (values: list uint256)
+                   (loc: string_map uint256)
+                   (Ok: L10.Interpret.bind_args names values = inr loc):
+  let _ := string_map_impl in
+     forall x,
+       match Map.lookup loc x with
+       | None => ~ In x names
+       | Some _ => In x names
+       end.
+Proof.
+revert values loc Ok. induction names as [|head_name], values as [|head_value]; try easy; intros.
+{ cbn in *. inversion Ok. subst. now rewrite Map.empty_lookup. }
+cbn in *.
+remember (Interpret.bind_args names values) as loc'. destruct loc' as [|loc']. { discriminate. }
+assert (IH := IHnames _ _ (eq_sym Heqloc') x).
+destruct (Map.lookup loc' head_name). { discriminate. }
+inversion Ok. subst. rewrite Map.insert_ok.
+destruct (string_dec head_name x).
+{ subst. left. trivial. }
+destruct (Map.lookup loc' x); tauto.
+Qed.
+
+Lemma bind_args_lt {C: VyperConfig}
+                   (names: list string)
+                   (values: list uint256)
+                   (L: length names < length values)
+                   (ND: NoDup names):
+   L10.Interpret.bind_args names values = inl "function called with too many arguments"%string.
+Proof.
+revert values L. induction names, values; intros; try easy.
+cbn.
+assert (ND': NoDup names) by now inversion ND.
+cbn in L. apply lt_S_n in L.
+now rewrite (IHnames ND' values L).
+Qed.
+
+Lemma bind_args_gt {C: VyperConfig}
+                   (names: list string)
+                   (values: list uint256)
+                   (G: length values < length names)
+                   (ND: NoDup names):
+   L10.Interpret.bind_args names values = inl "function called with too few arguments"%string.
+Proof.
+revert values G. induction names, values; intros; try easy.
+cbn.
+assert (ND': NoDup names) by now inversion ND.
+cbn in G. apply gt_S_n in G.
+now rewrite (IHnames ND' values G).
+Qed.
+
+Lemma bind_args_nodup {C: VyperConfig}
+                      (names: list string)
+                      (values: list uint256)
+                      (loc: string_map uint256)
+                      (Ok: L10.Interpret.bind_args names values = inr loc):
+  NoDup names.
+Proof.
+revert values loc Ok. induction names as [|head_name], values as [|head_value]; intros; try easy.
+{ constructor. }
+cbn in Ok.
+remember (Interpret.bind_args names values) as loc'. destruct loc' as [|loc']; try discriminate.
+remember (Map.lookup loc' head_name) as loc'_head. destruct loc'_head; try discriminate.
+constructor.
+{
+  assert (D := bind_args_domain _ _ _ (eq_sym Heqloc') head_name).
+  now rewrite<- Heqloc'_head in D.
+}
+exact (IHnames values loc' (eq_sym Heqloc')).
+Qed.
+
+Lemma bind_args_same_len {C: VyperConfig}
+                         (names: list string)
+                         (values: list uint256)
+                         (loc: string_map uint256)
+                         (Ok: L10.Interpret.bind_args names values = inr loc):
+  length names = length values.
+Proof.
+assert (T := Nat.lt_trichotomy (length names) (length values)).
+case T; clear T; intro T.
+{
+  rewrite bind_args_lt in Ok. { discriminate. } { assumption. }
+  apply (bind_args_nodup _ _ _ Ok).
+}
+case T; clear T; intro T. { assumption. }
+rewrite bind_args_gt in Ok. { discriminate. } { assumption. }
+apply (bind_args_nodup _ _ _ Ok).
+Qed.
+
+Lemma varmap_rec_ok {C: VyperConfig}
+                    (names: list string)
+                    (varmap: string_map N)
+                    (m: string_map N)
+                    (init: N)
+                    (Bound: VarsBound m init)
+                    (Inj: VarmapInj m)
+                    (Ok: make_varmap_rec m init names = inr varmap):
+  VarmapInj varmap /\ VarsBound varmap (init + N.of_nat (length names))%N.
+Proof.
+pose (empty  := @Map.empty  string string_dec N (@string_map C N) (@string_map_impl C N)).
+pose (insert := @Map.insert string string_dec N (@string_map C N) (@string_map_impl C N)).
+pose (lookup := @Map.lookup string string_dec N (@string_map C N) (@string_map_impl C N)).
+revert m init Bound Inj Ok. induction names; cbn; intros.
+{
+  assert (m = varmap) by now inversion Ok.
+  subst varmap. rewrite N.add_0_r. tauto.
+}
+remember (Map.lookup m a) as ma. destruct ma. { discriminate. }
+replace (init + N.pos (Pos.of_succ_nat (Datatypes.length names)))%N
+   with (N.succ init + N.of_nat (Datatypes.length names))%N by lia.
+refine (IHnames (insert m a init) (N.succ init) _ _ Ok).
+{
+  (* VarsBound (insert m a init) (N.succ init) *)
+  intro x.
+  unfold insert. rewrite Map.insert_ok.
+  assert (B := Bound x).
+  destruct (string_dec a x). { apply N.lt_succ_diag_r. }
+  destruct (Map.lookup m x) as [k|]. 2:trivial.
+  lia.
+}
+intros x y.
+unfold insert. repeat rewrite Map.insert_ok.
+destruct (string_dec a x).
+{
+  destruct (string_dec a y). { now subst. }
+  assert (B := Bound y).
+  destruct (Map.lookup m y) as [k|]. 2:trivial.
+  intro H. lia.
+}
+destruct (string_dec a y).
+{
+  assert (B := Bound x).
+  destruct (Map.lookup m x) as [k|]. 2:trivial.
+  intro H. lia.
+}
+apply Inj.
+Qed.
+
+Lemma varmap_ok {C: VyperConfig}
+                (names: list string)
+                (varmap: string_map N)
+                (Ok: make_varmap names = inr varmap):
+  VarmapInj varmap /\ VarsBound varmap (N.of_nat (length names))%N.
+Proof.
+unfold make_varmap in *.
+pose (empty  := @Map.empty  string string_dec N (@string_map C N) (@string_map_impl C N)).
+assert (R := varmap_rec_ok names varmap empty 0%N).
+cbn in R. apply R.
+{ (* VarsBound empty 0 *) intro x. unfold empty. now rewrite Map.empty_lookup. }
+{ (* VarmapInj empty *) intros x y. unfold empty. now rewrite Map.empty_lookup. }
+apply Ok.
+Qed.
+
+Lemma varmap_rec_mono {C: VyperConfig}
+                      (names: list string)
+                      (m varmap: string_map N)
+                      (init: N)
+                      (VarmapOk: make_varmap_rec m init names = inr varmap)
+                      (x: string):
+  let _ := string_map_impl in
+  match Map.lookup m x with
+  | Some y => Map.lookup varmap x = Some y
+  | None => True
+  end.
+Proof.
+revert m init VarmapOk.
+induction names as [|head]; intros; cbn in *.
+{ inversion VarmapOk. subst varmap. now destruct Map.lookup. }
+remember (Map.lookup m head) as m_head. destruct m_head. { discriminate. }
+assert (IH := IHnames _ _ VarmapOk).
+rewrite Map.insert_ok in IH.
+destruct (string_dec head x).
+{ subst. now destruct (Map.lookup m x). }
+apply IH.
+Qed.
+
+Local Lemma varmap_rec_index {C: VyperConfig}
+                             (names: list string)
+                             (m varmap: string_map N)
+                             (init: N)
+                             (VarmapOk: make_varmap_rec m init names = inr varmap)
+                             (x: string):
+  let _ := string_map_impl in
+  match Map.lookup m x, Map.lookup varmap x with
+  | None, Some index => (init <= index)%N /\ nth_error names (N.to_nat (index - init)%N) = Some x
+  | _, _ => ~ In x names
+  end.
+Proof.
+revert m varmap init VarmapOk x. induction names as [|head]; intros; cbn in *.
+{
+  inversion VarmapOk; subst varmap.
+  now destruct (Map.lookup m x).
+}
+remember (Map.lookup m head) as m_head. destruct m_head. { discriminate. }
+assert (IH := IHnames _ _ _ VarmapOk x).
+rewrite Map.insert_ok in IH.
+destruct (string_dec head x).
+{
+  subst head.
+  destruct (Map.lookup m x). { discriminate. }
+  assert (V := varmap_rec_mono _ _ _ _ VarmapOk x).
+  cbn in V. rewrite Map.insert_ok in V.
+  destruct (string_dec x x). 2:tauto.
+  destruct (Map.lookup varmap x). 2:discriminate.
+  inversion V. subst.
+  rewrite N.sub_diag.
+  split. { lia. }
+  trivial.
+}
+destruct (Map.lookup m x). { tauto. }
+destruct (Map.lookup varmap x) as [k|]. 2:tauto.
+remember (N.to_nat (k - N.succ init)) as a.
+remember (N.to_nat (k - init)) as b.
+destruct IH as (Bound, E).
+assert (B: b = S a) by lia.
+rewrite B.
+cbn.
+split. 2:assumption.
+lia.
+Qed.
+
+Lemma varmap_index {C: VyperConfig}
+                   (names: list string)
+                   (varmap: string_map N)
+                   (VarmapOk: make_varmap names = inr varmap)
+                   (x: string):
+  let _ := string_map_impl in
+  match Map.lookup varmap x with
+  | Some index => nth_error names (N.to_nat index) = Some x
+  | None => ~ In x names
+  end.
+Proof.
+unfold make_varmap in VarmapOk.
+cbn.
+assert (R := varmap_rec_index _ _ _ _ VarmapOk x). cbn in R.
+rewrite Map.empty_lookup in R.
+destruct (Map.lookup varmap x). 2:tauto.
+rewrite N.sub_0_r in R.
+tauto.
+Qed.
+
+Lemma bind_args_index {C: VyperConfig}
+                      (names: list string)
+                      (values: list uint256)
+                      (loc: string_map uint256)
+                      (LocOk: L10.Interpret.bind_args names values = inr loc)
+                      (index: nat)
+                      (x: string)
+                      (Ok: nth_error names index = Some x):
+  let _ := string_map_impl in
+  Map.lookup loc x = nth_error values index.
+Proof.
+cbn. revert index values loc LocOk Ok.
+induction names as [|head_name], values as [|head_value]; intros; try easy.
+{
+  assert (Oops: index < @length string nil).
+  { apply nth_error_Some. intro H. rewrite H in Ok. discriminate. }
+  cbn in Oops.
+  now apply Nat.nlt_0_r in Oops.
+}
+assert (F := bind_args_nodup _ _ _ LocOk).
+cbn in LocOk.
+remember (Interpret.bind_args names values) as loc'.
+destruct loc' as [|loc']. { discriminate. }
+remember (Map.lookup loc' head_name) as loc'_head. destruct loc'_head. { discriminate. }
+symmetry in Heqloc'.
+inversion LocOk. subst.
+rewrite Map.insert_ok.
+destruct index as [|index'].
+{
+  cbn in *. inversion Ok. subst.
+  destruct (string_dec x x); tauto.
+}
+cbn in *.
+rewrite<- (IHnames _ _ _ Heqloc' Ok).
+destruct (string_dec head_name x). 2:trivial.
+subst.
+apply nth_error_In in Ok.
+inversion F. contradiction.
+Qed.
+
+Lemma bind_varmap_agree {C: VyperConfig}
+                        (names: list string)
+                        (values: list uint256)
+                        (varmap: string_map N)
+                        (loc: string_map uint256)
+                        (VarmapOk: make_varmap names = inr varmap)
+                        (LocOk: L10.Interpret.bind_args names values = inr loc):
+  let _ := memory_impl in
+  VarsAgree varmap loc (OpenArray.from_list values).
+Proof.
+cbn. intro x.
+assert (V := varmap_index _ _ VarmapOk x). cbn in V.
+assert (D := bind_args_domain _ _ _ LocOk x).
+remember (Map.lookup varmap x) as varmap_x.
+destruct varmap_x. 2:now destruct (Map.lookup loc x).
+rewrite OpenArray.from_list_ok.
+assert (W := bind_args_index _ _ _ LocOk _ _ V). cbn in W.
+rewrite W in *.
+assert (L := bind_args_same_len _ _ _ LocOk).
+assert (BN: N.to_nat n < length names).
+{ apply nth_error_Some. rewrite V. discriminate. }
+assert (BV: N.to_nat n < length values). { rewrite<- L. apply BN. }
+remember (nth_error values (N.to_nat n)) as z. symmetry in Heqz. destruct z.
+2:{ apply nth_error_Some in BV. contradiction. }
+apply nth_error_nth with (d := uint256_of_Z 0) in Heqz. exact Heqz.
+Qed.
+
+Lemma interpret_translated_call {C: VyperConfig}
+                                (builtins: string -> option builtin)
+                                {cd20: L20.Descend.calldag}
+                                {call_depth_bound: nat}
+                                (fc: fun_ctx cd20 call_depth_bound)
+                                {cd30: L30.Descend.calldag}
+                                (ok: translate_calldag cd20 = inr cd30)
+                                (world: world_state)
+                                (arg_values: list uint256):
+  L30.Interpret.interpret_call builtins (translate_fun_ctx fc ok) world arg_values
+   =
+  L20.Interpret.interpret_call builtins fc world arg_values.
+Proof.
+revert world arg_values. induction call_depth_bound.
+{ exfalso. exact (Nat.nlt_0_r _ (proj1 (Nat.ltb_lt _ _) (fun_bound_ok fc))). }
+assert(F: inr (cached_translated_decl fc ok)
+           =
+          translate_decl (fun_decl fc)).
+{
+  clear IHcall_depth_bound.
+  unfold translate_fun_ctx in *. cbn in *.
+  unfold cached_translated_decl in *.
+  remember (FunCtx.translate_fun_ctx_fun_decl_helper fc ok) as foo. clear Heqfoo.
+  remember (cd_declmap cd30 (fun_name fc)) as d.
+  destruct d. 2:{ contradiction. }
+  subst.
+  assert (Q := translate_fun_ctx_declmap ok (fun_name fc)).
+  destruct (cd_declmap cd30 (fun_name fc)) as [d'|]. 2:discriminate.
+  inversion Heqd. subst d'. clear Heqd.
+  remember (cd_declmap cd20 (fun_name fc)) as x.
+  destruct x as [x|]. 2:discriminate.
+  inversion Q. f_equal.
+  assert (D := fun_decl_ok fc).
+  rewrite D in *. inversion Heqx.
+  trivial.
+}
+intros.
+cbn.
+remember (fun name arity body
+              (E: cached_translated_decl fc ok = AST.FunDecl name arity body) =>
+          if Datatypes.length arg_values =? N.to_nat arity
+          then
+           let
+           '(world', _, result) :=
+            Stmt.interpret_stmt eq_refl (translate_fun_ctx fc ok) (Interpret.interpret_call builtins)
+              builtins world (OpenArray.from_list arg_values) body (Interpret.interpret_call_helper E) in
+            (world',
+            match result with
+            | StmtSuccess => ExprSuccess zero256
+            | StmtAbort a => ExprAbort a
+            | StmtReturnFromFunction x => ExprSuccess x
+            end)
+          else (world,
+     expr_error
+       (if match N.to_nat arity with
+           | 0 => false
+           | S m' => Datatypes.length arg_values <=? m'
+           end
+        then "function called with too few arguments"%string
+        else "function called with too many arguments"%string))) as branch_30.
+remember (fun name arg_names body
+              (E : fun_decl fc = L20.AST.FunDecl name arg_names body) =>
+            match Interpret.bind_args arg_names arg_values with
+            | inl err => (world, expr_error err)
+            | inr loc =>
+                let
+                '(world', _, result) :=
+                 L20.Stmt.interpret_stmt eq_refl fc (L20.Interpret.interpret_call builtins) builtins world loc
+                   body (L20.Interpret.interpret_call_helper E) in
+                 (world',
+                 match result with
+                 | StmtSuccess => ExprSuccess zero256
+                 | StmtAbort a => ExprAbort a
+                 | StmtReturnFromFunction x => ExprSuccess x
+                 end)
+            end) as branch_20.
+assert (B: forall name arg_names body30 body20 E30 E20,
+             branch_30 name (N.of_nat (List.length arg_names)) body30 E30
+              =
+             branch_20 name arg_names body20 E20).
+{
+  intros. subst. rewrite Nat2N.id. rewrite E20 in F. rewrite E30 in F. cbn in F.
+  remember (make_varmap arg_names) as maybe_varmap.
+  destruct maybe_varmap as [err|varmap]. { discriminate. }
+  (* argument names have no duplication because translation would have failed *)
+  assert (ND: NoDup arg_names).
+  { apply varmap_nodup. intro err. rewrite<- Heqmaybe_varmap. discriminate. }
+
+  (* arity check *)
+  assert (T := Nat.lt_trichotomy (length arg_names) (length arg_values)).
+  case T; clear T; intro T.
+  {
+    replace (length arg_values =? length arg_names) with false.
+    2:{ symmetry. rewrite Nat.eqb_neq. apply Nat.neq_sym. apply Nat.lt_neq. exact T. }
+    replace (match length arg_names with
+             | 0 => false
+             | S m' => length arg_values <=? m'
+             end) with (length arg_values <? length arg_names) by trivial.
+    replace (length arg_values <? length arg_names) with false.
+    2:{ symmetry. rewrite Nat.ltb_ge. apply Nat.lt_le_incl. exact T. }
+    now rewrite (bind_args_lt _ _ T ND).
+  }
+  case T; clear T; intro T.
+  2:{
+    replace (length arg_values =? length arg_names) with false.
+    2:{ symmetry. rewrite Nat.eqb_neq. apply Nat.lt_neq. exact T. }
+    replace (match length arg_names with
+         | 0 => false
+         | S m' => length arg_values <=? m'
+         end) with (length arg_values <? length arg_names) by trivial.
+    assert (G := T).
+    rewrite<- Nat.ltb_lt in T. rewrite T.
+    now rewrite (bind_args_gt _ _ G ND).
+  }
+  assert (SameLen := T).
+  symmetry in T. rewrite<- Nat.eqb_eq in T. rewrite T. clear T.
+
+  assert (BindArgsOk := bind_args_domain_if_nodup arg_names arg_values SameLen ND).
+  remember (Interpret.bind_args arg_names arg_values) as loc.
+  destruct loc as [err|loc]. { contradiction. }
+  destruct (varmap_ok arg_names varmap (eq_sym Heqmaybe_varmap)) as (Inj, Bound).
+  remember (translate_stmt varmap (N.of_nat (Datatypes.length arg_names)) body20) as body30'.
+  destruct body30'. { discriminate. }
+  inversion F. subst.
+  assert (IS := interpret_translated_stmt eq_refl builtins fc ok
+                                          IHcall_depth_bound world loc
+                                          (OpenArray.from_list arg_values)
+                                          varmap Inj _
+                                          (bind_varmap_agree _ _ _ _
+                                            (eq_sym Heqmaybe_varmap)
+                                            (eq_sym Heqloc))
+                                          Bound
+                                          (eq_sym Heqbody30')
+                                          (L30.Interpret.interpret_call_helper E30)
+                                          (L20.Interpret.interpret_call_helper E20)).
+  cbn in IS.
+  destruct L30.Stmt.interpret_stmt as ((world30, mem30), result30).
+  destruct L20.Stmt.interpret_stmt as ((world20, loc20), result20).
+  destruct IS as (R, (W, Agree)).
+  subst.
+  trivial.
+}
+clear Heqbranch_20. clear Heqbranch_30.
+destruct (fun_decl fc); cbn in F.
+{ (* [fun_decl fc] is a global var *) now destruct cached_translated_decl. }
+destruct (make_varmap args). { discriminate. }
+destruct (translate_stmt s (N.of_nat (Datatypes.length args)) body). { discriminate. }
+inversion F.
+destruct (cached_translated_decl fc ok). { discriminate. }
+inversion H0 (* XXX *). subst.
+apply B.
+Qed.
+
+Lemma make_fun_ctx_and_bound_ok {C: VyperConfig}
+                                (cd20: L20.Descend.calldag)
+                                (cd30: L30.Descend.calldag)
+                                (Ok: translate_calldag cd20 = inr cd30)
+                                (fun_name: string):
+   make_fun_ctx_and_bound cd30 fun_name
+    =
+   match make_fun_ctx_and_bound cd20 fun_name with
+   | Some (existT _ bound fc) => Some (existT _ bound (translate_fun_ctx fc Ok))
+   | None => None
+   end.
+Proof.
+(* this is too complicated due to destructing convoys *)
+unfold make_fun_ctx_and_bound.
+remember (fun d (Ed : cd_declmap cd30 fun_name = Some d) =>
+    match
+      cd_depthmap cd30 fun_name as depth'
+      return (cd_depthmap cd30 fun_name = depth' -> option {bound : nat & fun_ctx cd30 bound})
+    with
+    | Some depth =>
+        fun Edepth : cd_depthmap cd30 fun_name = Some depth =>
+        Some
+          (existT (fun bound : nat => fun_ctx cd30 bound) (S depth)
+             {|
+             fun_name := fun_name;
+             fun_depth := depth;
+             fun_depth_ok := Edepth;
+             fun_decl := d;
+             fun_decl_ok := Ed;
+             fun_bound_ok := proj2 (Nat.ltb_lt depth (S depth)) (Nat.lt_succ_diag_r depth) |})
+    | None =>
+        fun Edepth : cd_depthmap cd30 fun_name = None =>
+        False_rect (option {bound : nat & fun_ctx cd30 bound}) (Calldag.make_fun_ctx_helper Ed Edepth)
+    end eq_refl) as lhs_some_branch.
+remember (fun d (Ed : cd_declmap cd20 fun_name = Some d) =>
+      match
+        cd_depthmap cd20 fun_name as depth'
+        return (cd_depthmap cd20 fun_name = depth' -> option {bound : nat & fun_ctx cd20 bound})
+      with
+      | Some depth =>
+          fun Edepth : cd_depthmap cd20 fun_name = Some depth =>
+          Some
+            (existT (fun bound : nat => fun_ctx cd20 bound) (S depth)
+               {|
+               fun_name := fun_name;
+               fun_depth := depth;
+               fun_depth_ok := Edepth;
+               fun_decl := d;
+               fun_decl_ok := Ed;
+               fun_bound_ok := proj2 (Nat.ltb_lt depth (S depth)) (Nat.lt_succ_diag_r depth) |})
+      | None =>
+          fun Edepth : cd_depthmap cd20 fun_name = None =>
+          False_rect (option {bound : nat & fun_ctx cd20 bound})
+            (Calldag.make_fun_ctx_helper Ed Edepth)
+      end eq_refl) as rhs_some_branch.
+enough (SomeBranchOk: forall d30 d20 Ed30 Ed20
+                             (DeclOk: translate_decl d20 = inr d30),
+                        lhs_some_branch d30 Ed30
+                         =
+                        match rhs_some_branch d20 Ed20 with
+                        | Some (existT _ bound fc) =>
+                            Some
+                              (existT _ bound
+                                 (translate_fun_ctx fc Ok))
+                        | None => None
+                        end).
+{
+  cbn in *.
+  remember (fun _: _ = None => None) as lhs_none_branch.
+  assert (NoneBranchOk: forall E, lhs_none_branch E = None).
+  { subst. trivial. }
+  clear Heqlhs_some_branch Heqrhs_some_branch Heqlhs_none_branch.
+  assert (T := translate_fun_ctx_declmap Ok fun_name).
+  destruct (cd_declmap cd20 fun_name); destruct (cd_declmap cd30 fun_name);
+    try easy.
+  apply SomeBranchOk.
+  now inversion T.
+}
+subst. cbn. intros.
+
+(* This is even more messed up than usual because just the implicit arguments weren't enough. *)
+remember (fun depth
+       (Edepth : @eq (option nat)
+                    (@cd_depthmap C (@AST.decl C) (@Callset.decl_callset C) cd30 fun_name)
+                    (@Some nat depth)) =>
+       @Some
+         (@sigT nat (fun bound : nat => @fun_ctx C (@AST.decl C) (@Callset.decl_callset C) cd30 bound))
+         (@existT nat
+            (fun bound : nat => @fun_ctx C (@AST.decl C) (@Callset.decl_callset C) cd30 bound)
+            (S depth)
+            _))
+  as depth_lhs_some_branch.
+remember (fun (depth: nat)
+        (Edepth: cd_depthmap cd20 fun_name = Some depth) =>
+      Some
+        (existT (fun bound : nat => fun_ctx cd20 bound) (S depth)
+           _))
+  as depth_rhs_some_branch.
+enough (A: forall depth E30 E20,
+          depth_lhs_some_branch depth E30
+           =
+          match depth_rhs_some_branch depth E20 with
+          | Some (existT _ bound fc) =>
+              Some
+                (existT (fun bound0 : nat => fun_ctx cd30 bound0) bound
+                   (translate_fun_ctx fc Ok))
+          | None => None
+          end).
+{
+  clear Heqdepth_lhs_some_branch Heqdepth_rhs_some_branch.
+  remember (fun Edepth : cd_depthmap cd30 fun_name = None =>
+      False_rect (option {bound : nat & fun_ctx cd30 bound}) (Calldag.make_fun_ctx_helper Ed30 Edepth))
+    as lhs_none_branch.
+  remember (fun Edepth : cd_depthmap cd20 fun_name = None =>
+        False_rect (option {bound : nat & fun_ctx cd20 bound}) (Calldag.make_fun_ctx_helper Ed20 Edepth))
+    as rhs_none_branch.
+  clear Heqlhs_none_branch Heqrhs_none_branch.
+  assert (Guard30 := Calldag.make_fun_ctx_helper Ed30).
+  assert (Guard20 := Calldag.make_fun_ctx_helper Ed20).
+  assert (T := translate_fun_ctx_depthmap Ok fun_name).
+  destruct (cd_depthmap cd30 fun_name), (cd_depthmap cd20 fun_name); try easy.
+  inversion T. subst.
+  apply A.
+}
+intros. subst.
+f_equal. f_equal.
+unfold translate_fun_ctx. cbn.
+assert (FunCtxEq: forall name1 depth depth_ok1 decl1 decl_ok1 bound_ok1
+                         name2       depth_ok2 decl2 decl_ok2 bound_ok2
+                         (Name: name1 = name2)
+                         (Decl: decl1 = decl2),
+  ({| fun_name := name1
+    ; fun_depth := depth
+    ; fun_depth_ok := depth_ok1
+    ; fun_decl := decl1
+    ; fun_decl_ok := decl_ok1
+    ; fun_bound_ok := bound_ok1 |}: fun_ctx cd30 (S depth))
+   =
+  {| fun_name := name2
+   ; fun_depth := depth
+   ; fun_depth_ok := depth_ok2
+   ; fun_decl := decl2
+   ; fun_decl_ok := decl_ok2
+   ; fun_bound_ok := bound_ok2 |}).
+{
+  intros. subst.
+  assert (depth_ok1 = depth_ok2) by apply PropExtensionality.proof_irrelevance.
+  assert (decl_ok1 = decl_ok2) by apply PropExtensionality.proof_irrelevance.
+  assert (bound_ok1 = bound_ok2) by apply PropExtensionality.proof_irrelevance.
+  subst.
+  trivial.
+}
+apply FunCtxEq. { (* name: *) trivial. }
+clear FunCtxEq.
+assert (Unsome: forall {T} (x y: T), Some x = Some y -> x = y).
+{ intros T x y H. now inversion H. }
+apply Unsome.
+rewrite<- FunCtx.translate_fun_ctx_decl_ok. cbn. symmetry. exact Ed30.
+Qed.
+
+Theorem translate_ok {C: VyperConfig}
+                     (builtins: string -> option builtin)
+                     (cd20: L20.Descend.calldag)
+                     (cd30: L30.Descend.calldag)
+                     (Ok: translate_calldag cd20 = inr cd30)
+                     (fun_name: string)
+                     (world: world_state)
+                     (arg_values: list uint256):
+  L30.Interpret.interpret builtins cd30 fun_name world arg_values
+   =
+  L20.Interpret.interpret builtins cd20 fun_name world arg_values.
+Proof.
+unfold L20.Interpret.interpret. unfold L30.Interpret.interpret.
+rewrite (make_fun_ctx_and_bound_ok cd20 cd30 Ok).
+destruct (make_fun_ctx_and_bound cd20 fun_name) as [(bound, fc)|]; cbn.
+{ apply interpret_translated_call. }
+trivial.
+Qed.
